generic/Zeta.Generic.Thread.fsti
@@ -1,0 +1,63 @@
+module Zeta.Generic.Thread
+
+open Zeta.GenericVerifier
+open Zeta.Time
+
+module S = FStar.Seq
+module SA = Zeta.SeqAux
+
+(* a verifier log attached to a thread id *)
+let tid_vlog (vspec: verifier_spec) = thread_id & verifier_log vspec
+
+let length #vspec (tl: tid_vlog vspec) =
+  let _, l = tl in
+  S.length l
+
+let seq_index #vspec (tl: tid_vlog vspec) = i:nat {i < length tl}
+
+let index #vspec (tl: tid_vlog vspec) (i: seq_index tl) =
+  let _, l = tl in
+  S.index l i
+
+let prefix #vspec (tl: tid_vlog vspec) (i: nat {i <= length tl}): tid_vlog _ =
+  let tid, l = tl in
+  tid, SA.prefix l i
+
+let verify #vspec (tl: tid_vlog vspec): vspec.vtls_t =
+  let tid, l = tl in
+  Zeta.GenericVerifier.verify tid l
+
+let verifiable #vspec (tl: tid_vlog vspec) = vspec.valid (verify tl)
+
+let verifiable_log vspec = tl: tid_vlog vspec { verifiable tl }
+
+(* if a thread log is verifiable, its prefix is verifiable *)
+val verifiable_implies_prefix_verifiable (#vspec:verifier_spec)
+  (tl:verifiable_log vspec) (i:nat{i <= length tl}):
+  Lemma (ensures (verifiable (prefix tl i)))
+        [SMTPat (prefix tl i)]
+
+(* clock after processing i entries of the log *)
+let clock #vspec (tl: verifiable_log vspec) (i: nat { i <= length tl }) =
+  vspec.clock (verify tl)
+
+(* clock is monotonic *)
+val lemma_clock_monotonic (#vspec:verifier_spec)
+  (tl: verifiable_log vspec) (i:nat) (j:nat {j >= i /\ j <= length tl}):
+  Lemma (clock tl i `ts_leq` clock tl j)
+
+(* the thread id in the state is always the one specified in the parameter *)
+val lemma_thread_id_state (#vspec:verifier_spec) (tl: verifiable_log vspec):
+  Lemma (ensures (let tid, _ = tl in
+                  vspec.tid (verify tl) = tid))
+
+(* the verifier state after processing i entries *)
+let state_at #vspec (tl: verifiable_log vspec) (i:nat{i <= length tl}) =
+  (verify (prefix tl i))
+
+(* the state after processing i'th entry is obtained by applying the verify
+ * step to the state before processing the i'th entry *)
+val lemma_state_transition (#vspec:verifier_spec) (tl: verifiable_log vspec) (i: seq_index tl):
+  Lemma (ensures (state_at tl (i + 1) ==
+                  verify_step (index tl i) (state_at tl i)))
+        [SMTPat (verify_step (index tl i) (state_at tl i))]
